MutualExclusion specified

peterson.dfy
@@ -2,13 +2,15 @@ datatype Process = 0 | 1;
 datatype CState =  a1 | a2 | a3a | a3b | cs | a4;
 datatype State = State(pc: Process -> CState, flag: Process -> bool, turn: Process)
 
-var pc : Process -> CState;
-var flag : Process -> bool;
-var turn;
+const P : set <Process>
 
 function Other(p: process) : Process
 {
     if p == 0 then 1 else 0
+}
+
+predicate Valid(s: State) {
+    s.flag.Keys == s.pc.Keys == P
 }
 
 predicate Init(s: State) {
@@ -17,43 +19,68 @@ predicate Init(s: State) {
     s.pc(0) == s.pc(1) == a1
 }
 
+predicate Next(s: State, s': State) {
+    Valid(s) &&
+    exists p : Process :: p in P && NextP(p, s, s')
+}
+
+predicate NextP(p: Process, s: State, s': State)
+requires Valid(s) && p in P
+{
+    a1(p, s, s') ||
+    a2(p, s, s') ||
+    a3a(p, s, s') ||
+    a3b(p, s, s') ||
+    cs(p, s, s') ||
+    a4(p, s, s')
+}
+
 predicate a1(p: Process, s: State, s': State) 
-requires s.pc(p) == a1
+requires p in P && Valid(s) && s.pc(p) == a1
 {
     s'.flag(p) == true &&
     s'.pc(p) == a2
 }
 
 predicate a2(p: Process, s: State, s': State) 
-requires s.pc(p) == a2
+requires p in P && Valid(s) && s.pc(p) == a2
 {
     s'.turn == Other(p) &&
     s'.pc(p) == a3a;
 }
 
 method a3a(p: Process, s: State, s': State) 
-requires s.pc(p) == a3a
+requires p in P && Valid(s) && s.pc(p) == a3a
 {
     (s.flag(Other(p)) && s'.pc(p) == a3b) ||
     (!s.flag(Other(p)) && s'.pc(p) == cs)
 }
 
 method a3b(p: Process, s: State, s': State) 
-requires s.pc(p) == a3b)
+requires p in P && Valid(s) && s.pc(p) == a3b)
 {
     (turn == Other(p) && s'.pc(p) == a3a) ||
     (turn != Other(p) && s'.pc(p) == cs)
 }
 
 method cs(p:Process, s: State, s': State) 
-requires s.pc(p) == cs)
+requires p in P && Valid(s) && s.pc(p) == cs)
 {
     s'.pc(p) == a4
 }
 
 method a4(p: Process, s: State, s': State) 
-requires s.pc(p) == a4) 
+requires p in P && Valid(s) && s.pc(p) == a4) 
 {
     s'.flag(p) == false &&
     s'.pc(p) == a1
+}
+
+// Mutual Exclusion
+lemma MutualExclusion(s: State, p: Process, q: Process)
+requires Valid(s)
+requires s.pc(p) == cs && s.pc(q) == cs
+ensures p == q
+{
+    
 }
